
#### 8.1 Derivative of $f(x)=2 x-7$.
8.1 Using the $\Delta$-definition, find the derivative $f^{\prime}(x)$ of the function $f(x)=2 x-7$.
?x
$$
\begin{aligned}
f(x+\Delta x)=2(x+\Delta x)-7=2 x+2 \Delta x-7 . \\
\quad
\text { So, } \quad f(x+\Delta x)-f(x)= \\
(2 x+2 \Delta x-7)-(2 x-7)=2 \Delta x .
\end{aligned}
$$


Hence, $\frac{f(x+\Delta x)-f(x)}{\Delta x}=2$. Thus, $f^{\prime}(x)=\lim _{\Delta x \rightarrow 0} \frac{f(x+\Delta x)-f(x)}{\Delta x}=\lim _{\Delta x \rightarrow 0} 2=2$. Answer

#### 8.2 Show that Derivative of any linear function
8.2 Using the $\Delta$-definition, show that the derivative of any linear function $f(x)=A x+B$ is $f^{\prime}(x)=A$.

??x
$$
\begin{aligned}
f(x+\Delta x)=A(x+\Delta x)+B=A x+A \Delta x+B .\\ 
\quad \text { Then, } \quad f(x+\Delta x)-f(x)=\\
(A x+A \Delta x+B)-(A x+B)=

\end{aligned}
$$
 
 
 $A \Delta x$. Hence, $\frac{f(x+\Delta x)-f(x)}{\Delta x}=A$. Thus, $f^{\prime}(x)=\lim _{\Delta x \rightarrow 0} \frac{f(x+\Delta x)-f(x)}{\Delta x}=\lim _{\Delta x \rightarrow 0} A=A$.

x??
#### 8.3 Find the derivative of $f(x)=2 x^2-3 x+5$.
8.3 Using the $\Delta$-definition, find the derivative $f^{\prime}(x)$ of the function $f(x)=2 x^2-3 x+5$.

??x

$$
\begin{aligned}
f(x+\Delta x)=2(x+\Delta x)^2-3(x+\Delta x)+5=\\
2\left[x^2+2 x \Delta x+(\Delta x)^2\right]-3 x-3 \Delta x+5=\\
2 x^2+4 x \Delta x+2(\Delta x)^2-f(x+\Delta x)-f(x)=\\
\left[2 x^2+4 x \Delta x+2(\Delta x)^2-3 x-3 \Delta x+5\right]-\left(2 x^2-3 x+5\right)=4 x \Delta x

\end{aligned}
$$

$3 x-3 \Delta x+5$. So, $+$ $2(\Delta x)^2-3 \Delta x=(\Delta x)(4 x+2 \Delta x-3)$. 

Thus, $\quad \frac{f(x+\Delta x)-f(x)}{\Delta x}=4 x+2 \Delta x-3$. Hence, $\quad f^{\prime}(x)=$ $\lim _{\Delta x \rightarrow 0} \frac{f(x+\Delta x)-f(x)}{\Delta x}=\lim _{\Delta x \rightarrow 0}(4 x+2 \Delta x-3)=4 x-3$.


x??
#### 8.4 Find the Derivative of $f(x)=x^3$.
8.4 Using the $\Delta$-definition, find the derivative $f^{\prime}(x)$ of the function $f(x)=x^3$.

??x

$$
f(x+\Delta x)=(x+\Delta x)^3=x^3+3 x^2 \Delta x+3 x(\Delta x)^2+(\Delta x)^3 . \quad \text { So, } \quad f(x+\Delta x)-f(x)=\left[x^3+3 x^2 \Delta x+3 x(\Delta x)^2+\right.
$$

$\left.(\Delta x)^3\right]-x^3=3 x^2 \Delta x+3 x(\Delta x)^2+(\Delta x)^3=(\Delta x)\left(3 x^2+3 x \Delta x+(\Delta x)^2\right) . \quad$ So, $\quad \frac{f(x+\Delta x)-f(x)}{\Delta x}=3 x^2+3 x \Delta x+$ $(\Delta x)^2$. Thus, $f^{\prime}(x)=\lim _{\Delta x \rightarrow 0} \frac{f(x+\Delta x)-f(x)}{\Delta x}=\lim _{\Delta x \rightarrow 0}\left[3 x^2+3 x \Delta x+(\Delta x)^2\right]=3 x^2$.

x??
